Start work on proof that reader only creates theorems
Show that running the reader will produce a reader state
which only consists of 'correct' types, terms and theorems.
Proved most trivial cases. Things are lacking in the
READER_STATE invariant; READER_STATE must be extended to
enforce OBJ for all objects in the dictionary.

candle/standard/opentheory/readerProofScript.sml
@@ -3,6 +3,25 @@ open preamble readerTheory ml_monadBaseTheory
 
 val _ = new_theory"readerProof";
 
+(* case_eq theorems *)
+
+val exc_case_eq = prove_case_eq_thm{case_def=exc_case_def,nchotomy=exc_nchotomy};
+val term_case_eq = prove_case_eq_thm{case_def=holSyntaxTheory.term_case_def,nchotomy=holSyntaxTheory.term_nchotomy};
+val option_case_eq = prove_case_eq_thm{case_def=optionTheory.option_case_def,nchotomy=optionTheory.option_nchotomy};
+val object_case_eq = prove_case_eq_thm{case_def=readerTheory.object_case_def,nchotomy=readerTheory.object_nchotomy};
+val exn_case_eq = prove_case_eq_thm{case_def=holKernelTheory.hol_exn_case_def,nchotomy=holKernelTheory.hol_exn_nchotomy};
+val list_case_eq = prove_case_eq_thm{case_def=listTheory.list_case_def,nchotomy=listTheory.list_nchotomy};
+val update_case_eq = prove_case_eq_thm{case_def=holSyntaxTheory.update_case_def,nchotomy=holSyntaxTheory.update_nchotomy};
+val state_case_eq = prove_case_eq_thm{case_def=readerTheory.state_case_def,nchotomy=readerTheory.state_nchotomy};
+val case_eq_thms =
+  LIST_CONJ
+    [exc_case_eq, term_case_eq, option_case_eq,
+     object_case_eq, list_case_eq, pair_case_eq,
+     exn_case_eq, update_case_eq, thm_caseeq,
+     hol_refs_caseeq,state_case_eq]
+
+(* --- Reader does not raise Clash --- *)
+
 val pop_not_clash = Q.store_thm("pop_not_clash[simp]",
   `pop x y ≠ (Failure (Clash tm),refs)`,
   EVAL_TAC \\ rw[] \\ EVAL_TAC);
@@ -77,6 +96,601 @@ val getTys_not_clash = Q.store_thm("getTys_not_clash[simp]",
   \\ every_case_tac \\ fs [] \\ rpt (pairarg_tac \\ fs [])
   \\ every_case_tac \\ fs [] \\ rw []
   \\ metis_tac [getName_not_clash, getType_not_clash, getPair_not_clash]);
+
+(* --- Use Candle kernel soundness theorem --- *)
+
+(* TODO replace with actual theorem *)
+val readLine_no_clash = Q.store_thm("readLine_no_clash[simp]",
+  `readLine line st refs <> (Failure (Clash tm), refs)`,
+  cheat
+  );
+
+(* Refinement invariant for objects *)
+val OBJ_def = tDefine "OBJ" `
+  (OBJ defs (List xs)     <=> EVERY (OBJ defs) xs) /\
+  (OBJ defs (Type ty)     <=> TYPE defs ty) /\
+  (OBJ defs (Var (n, ty)) <=> TYPE defs ty) /\
+  (OBJ defs (Term tm)     <=> TERM defs tm) /\
+  (OBJ defs (Thm thm)     <=> THM defs thm) /\
+  (OBJ defs _             <=> T)`
+  (WF_REL_TAC `measure (object_size o SND)`
+   \\ Induct \\ rw [object_size_def]
+   \\ res_tac \\ fs []);
+
+val READER_STATE_def = Define `
+  READER_STATE defs st <=>
+    EVERY (THM defs) st.thms /\
+    EVERY (OBJ defs) st.stack`
+
+val getNum_thm = Q.store_thm("getNum_thm",
+  `STATE defs refs /\
+   getNum obj refs = (res, refs')
+   ==>
+   STATE defs refs'`,
+   Cases_on `obj` \\ rw [getNum_def, raise_Fail_def, st_ex_return_def] \\ fs []);
+
+val getName_thm = Q.store_thm("getName_thm",
+  `STATE defs refs /\
+   getName obj refs = (res, refs')
+   ==>
+   STATE defs refs'`,
+   Cases_on `obj` \\ rw [getName_def, raise_Fail_def, st_ex_return_def] \\ fs []);
+
+val getList_thm = Q.store_thm("getList_thm",
+  `STATE defs refs /\
+   OBJ defs obj /\
+   getList obj refs = (res, refs')
+   ==>
+   STATE defs refs' /\
+   case res of
+     Failure _ => T
+   | Success ls => EVERY (OBJ defs) ls`,
+   Cases_on `obj` \\ rw [getList_def, raise_Fail_def, st_ex_return_def] \\ fs []
+   \\ metis_tac [OBJ_def]);
+
+val getTypeOp_thm = Q.store_thm("getTypeOp_thm",
+  `STATE defs refs /\
+   getTypeOp obj refs = (res, refs')
+   ==>
+   STATE defs refs'`,
+   Cases_on `obj` \\ rw [getTypeOp_def, raise_Fail_def, st_ex_return_def] \\ fs []);
+
+val getType_thm = Q.store_thm("getType_thm",
+  `STATE defs refs /\
+   OBJ defs obj /\
+   getType obj refs = (res, refs')
+   ==>
+   STATE defs refs' /\
+   case res of
+     Failure _ => T
+   | Success ty => TYPE defs ty`,
+   Cases_on `obj` \\ rw [getType_def, raise_Fail_def, st_ex_return_def]
+   \\ fs [OBJ_def]);
+
+val getConst_thm = Q.store_thm("getConst_thm",
+  `STATE defs refs /\
+   getConst obj refs = (res, refs')
+   ==>
+   STATE defs refs'`,
+   Cases_on `obj` \\ rw [getConst_def, raise_Fail_def, st_ex_return_def] \\ fs []);
+
+val getVar_thm = Q.store_thm("getVar_thm",
+  `STATE defs refs /\
+   OBJ defs obj /\
+   getVar obj refs = (res, refs')
+   ==>
+   STATE defs refs' /\
+   case res of
+     Failure _ => T
+   | Success (_, ty) => TYPE defs ty`,
+   Cases_on `obj` \\ rw [getVar_def, raise_Fail_def, st_ex_return_def] \\ fs []
+   \\ CASE_TAC \\ fs [OBJ_def]);
+
+val getTerm_thm = Q.store_thm("getTerm_thm",
+  `STATE defs refs /\
+   OBJ defs obj /\
+   getTerm obj refs = (res, refs')
+   ==>
+   STATE defs refs' /\
+   case res of
+     Failure _ => T
+   | Success tm => TERM defs tm`,
+   Cases_on `obj` \\ rw [getTerm_def, raise_Fail_def, st_ex_return_def] \\ fs []
+   \\ fs [OBJ_def]);
+
+val getThm_thm = Q.store_thm("getThm_thm",
+  `STATE defs refs /\
+   OBJ defs obj /\
+   getThm obj refs = (res, refs')
+   ==>
+   STATE defs refs' /\
+   case res of
+     Failure _ => T
+   | Success thm => THM defs thm`,
+   Cases_on `obj` \\ rw [getThm_def, raise_Fail_def, st_ex_return_def] \\ fs []
+   \\ fs [OBJ_def]);
+
+val pop_thm = Q.store_thm("pop_thm",
+  `STATE defs refs /\
+   READER_STATE defs st /\
+   pop st refs = (res, refs')
+   ==>
+   STATE defs refs' /\
+   case res of
+     Failure _ => T
+   | Success (a, st') => OBJ defs a /\ READER_STATE defs st'`,
+   rw [pop_def, raise_Fail_def, st_ex_return_def]
+   \\ every_case_tac \\ fs [READER_STATE_def, state_component_equality]);
+
+val peek_thm = Q.store_thm("peek_thm",
+  `STATE defs refs /\
+   READER_STATE defs st /\
+   peek st refs = (res, refs')
+   ==>
+   STATE defs refs' /\
+   case res of
+     Failure _ => T
+   | Success obj => OBJ defs obj`,
+   rw [peek_def, raise_Fail_def, st_ex_return_def]
+   \\ every_case_tac \\ fs []
+   \\ fs [READER_STATE_def]);
+
+val push_thm = Q.store_thm("push_thm",
+  `READER_STATE defs st /\
+   OBJ defs obj
+   ==>
+   READER_STATE defs (push obj st)`,
+  rw [push_def, READER_STATE_def]);
+
+(*val insert_dict_thm = Q.store_thm("insert_dict_thm",*)
+  (*`T`, cheat);*)
+
+(*val delete_dict_thm = Q.store_thm("delete_dict_thm",*)
+  (*`T`, cheat);*)
+
+val first_EVERY = Q.store_thm("first_EVERY",
+  `!Q xs x.
+     EVERY P xs /\
+     first Q xs = SOME x
+     ==>
+     P x`,
+  recInduct first_ind \\ rw [Once first_def]
+  \\ Cases_on `l` \\ fs [] >- fs [Once first_def]
+  \\ pop_assum mp_tac
+  \\ once_rewrite_tac [first_def]
+  \\ fs [bool_case_eq]
+  \\ strip_tac \\ fs []
+  \\ first_x_assum (qspec_then `x` mp_tac)
+  \\ CASE_TAC \\ fs [] >- fs [Once first_def]
+  \\ fs [bool_case_eq]
+  \\ once_rewrite_tac [first_def] \\ fs [bool_case_eq]
+  \\ CASE_TAC \\ fs []
+  >-
+   (fs [Once first_def]
+    \\ fs [case_eq_thms, bool_case_eq, Once first_def])
+  \\ fs [Once first_def, case_eq_thms, bool_case_eq]
+  \\ fs [Once first_def, case_eq_thms, bool_case_eq]
+  \\ fs [Once first_def, case_eq_thms, bool_case_eq]);
+
+val find_axiom_thm = Q.store_thm("find_axiom_thm",
+  `EVERY (THM defs) refs.the_axioms /\ (* this is nowhere to be found; can it be assumed? *)
+   STATE defs refs /\
+   EVERY (TERM defs) ls /\
+   TERM defs tm /\
+   find_axiom (ls, tm) refs = (res, refs')
+   ==>
+   STATE defs refs' /\
+   case res of
+     Failure _ => T
+   | Success thm => THM defs thm`,
+  fs [find_axiom_def, st_ex_bind_def, st_ex_return_def, raise_Fail_def]
+  \\ fs [get_the_axioms_def]
+  \\ every_case_tac \\ fs [] \\ rw [] \\ fs []
+  \\ qmatch_asmsub_abbrev_tac `first P`
+  \\ Q.ISPECL_THEN [`THM defs`, `P`] mp_tac (GEN_ALL first_EVERY)
+  \\ disch_then drule \\ fs []);
+
+val getPair_thm = Q.store_thm("getPair_thm",
+  `STATE defs refs /\
+   OBJ defs obj /\
+   getPair obj refs = (res, refs')
+   ==>
+   STATE defs refs' /\
+   case res of
+     Failure _ => T
+   | Success (a, b) => OBJ defs a /\ OBJ defs b`,
+  Cases_on `obj` \\ rw [getPair_def, st_ex_return_def, raise_Fail_def] \\ fs []
+  \\ Cases_on `l` \\ fs [getPair_def, st_ex_return_def, raise_Fail_def] \\ rfs []
+  \\ every_case_tac \\ fs []
+  \\ Cases_on `t` \\ fs [getPair_def, st_ex_return_def, raise_Fail_def]
+  \\ rename1 `x::y::z`
+  \\ Cases_on `z` \\ fs [getPair_def, st_ex_return_def, raise_Fail_def]
+  \\ fs [OBJ_def]);
+
+val getTys_thm = Q.store_thm("getTys_thm",
+  `STATE defs refs /\
+   OBJ defs obj /\
+   getTys obj refs = (res, refs')
+   ==>
+   STATE defs refs' /\
+   case res of
+     Failure _ => T
+   | Success (t, ty) => TYPE defs t /\ TYPE defs ty`,
+  Cases_on `obj`
+  \\ fs [getTys_def, st_ex_bind_def, st_ex_return_def, raise_Fail_def, UNCURRY]
+  \\ every_case_tac \\ fs [] \\ rw [] \\ fs []
+  \\ TRY (fs [getPair_def, st_ex_return_def, raise_Fail_def] \\ NO_TAC)
+  \\ TRY (PairCases_on `a`) \\ fs []
+  \\ TRY (map_every imp_res_tac [getPair_thm, getType_thm, getName_thm] \\ fs [] \\ NO_TAC)
+  \\ fs [STATE_def]
+  \\ irule mk_vartype_thm
+  \\ fs [STATE_def] \\ rfs []);
+
+val getTms_thm = Q.store_thm("getTms_thm",
+  `STATE defs refs /\
+   OBJ defs obj /\
+   getTms obj refs = (res, refs')
+   ==>
+   STATE defs refs' /\
+   case res of
+     Failure _ => T
+   | Success (tm, var) => TERM defs tm /\ TERM defs var`,
+  Cases_on `obj`
+  \\ fs [getTms_def, st_ex_bind_def, st_ex_return_def, raise_Fail_def, UNCURRY]
+  \\ every_case_tac \\ fs [] \\ rw [] \\ fs []
+  \\ TRY (fs [getPair_def, st_ex_return_def, raise_Fail_def] \\ NO_TAC)
+  \\ TRY (PairCases_on `a`) \\ fs []
+  \\ TRY (map_every imp_res_tac [getPair_thm, getTerm_thm, getVar_thm] \\ fs [] \\ NO_TAC)
+  \\ rename1 `getVar _ _ = (_ v,_)` \\ PairCases_on `v`
+  \\ irule mk_var_thm >- (asm_exists_tac \\ fs [])
+  \\ map_every imp_res_tac [getPair_thm, getTerm_thm, getVar_thm] \\ fs []);
+
+val getNvs_thm = Q.store_thm("getNvs_thm",
+  `STATE defs refs /\
+   OBJ defs obj /\
+   getNvs obj refs = (res, refs')
+   ==>
+   STATE defs refs' /\
+   case res of
+     Failure _ => T
+   | Success (v1, v2) => TERM defs v1 /\ TERM defs v2`,
+  Cases_on `obj`
+  \\ fs [getNvs_def, st_ex_bind_def, st_ex_return_def, raise_Fail_def, UNCURRY]
+  \\ every_case_tac \\ fs [] \\ rw [] \\ fs []
+  \\ TRY (fs [getPair_def, st_ex_return_def, raise_Fail_def] \\ NO_TAC)
+  \\ TRY (PairCases_on `a`) \\ fs []
+  \\ TRY (map_every imp_res_tac [getPair_thm, getName_thm, getVar_thm] \\ fs [] \\ NO_TAC)
+  \\ rename1 `getVar _ _ = (_ v,_)` \\ PairCases_on `v`
+  \\ irule mk_var_thm
+  \\ TRY (asm_exists_tac \\ fs [])
+  \\ map_every imp_res_tac [getPair_thm, getName_thm, getVar_thm] \\ fs []);
+
+val getCns_thm = Q.store_thm("getCns_thm",
+  `STATE defs refs /\
+   TERM defs tm /\
+   getCns (tm, _) refs = (res, refs')
+   ==>
+   STATE defs refs' /\
+   case res of
+     Failure _ => T
+   | Success a => OBJ defs a`,
+  rw [getCns_def, st_ex_bind_def, st_ex_return_def, UNCURRY]
+  \\ every_case_tac \\ fs [] \\ rw []
+  \\ metis_tac [dest_var_thm, OBJ_def]);
+
+(* TODO remove: EQ_MP_thm *)
+val EQ_MP_STATE = Q.store_thm("EQ_MP_STATE",
+  `STATE defs refs /\
+   EQ_MP th1 th2 refs = (res, refs')
+   ==>
+   STATE defs refs'`,
+   Cases_on `th1` \\ Cases_on `th2`
+   \\ fs [EQ_MP_def, raise_Fail_def, st_ex_return_def]
+   \\ every_case_tac \\ fs [] \\ rw [] \\ fs []);
+
+val readLine_thm = Q.store_thm("readLine_thm",
+  `STATE defs refs /\
+   READER_STATE defs st /\
+   readLine line st refs = (res, refs')
+   ==>
+   STATE defs refs' /\
+   case res of
+     Failure _ => T
+   | Success st' => READER_STATE defs st'`,
+
+  fs [readLine_def, st_ex_bind_def, st_ex_return_def, raise_Fail_def]
+  \\ IF_CASES_TAC \\ fs []
+  >- (* version *)
+   (fs [case_eq_thms] \\ rw []
+    \\ TRY (pairarg_tac \\ fs []) \\ fs [case_eq_thms] \\ rw []
+    \\ map_every imp_res_tac [getNum_thm, pop_thm] \\ fs [])
+  \\ IF_CASES_TAC \\ fs []
+  >- (* absTerm *)
+    cheat
+  \\ IF_CASES_TAC \\ fs []
+  >- (* absThm *)
+    cheat
+  \\ IF_CASES_TAC \\ fs []
+  >- (* appTerm *)
+   (
+    fs [case_eq_thms] \\ rw []
+    \\ TRY (pairarg_tac \\ fs []) \\ fs [case_eq_thms]
+    \\ TRY (pairarg_tac \\ fs []) \\ fs [case_eq_thms] \\ rw []
+    \\ cheat (* TODO mk_comb *)
+   )
+  \\ IF_CASES_TAC \\ fs []
+  >- (* appThm *)
+   (
+    fs [case_eq_thms] \\ rw  []
+    \\ TRY (pairarg_tac \\ fs []) \\ fs [case_eq_thms]
+    \\ TRY (pairarg_tac \\ fs []) \\ fs [case_eq_thms] \\ rw []
+    \\ cheat (* TODO MK_COMB *)
+   )
+  \\ IF_CASES_TAC \\ fs []
+  >- (* assume *)
+   (
+    fs [case_eq_thms] \\ rw []
+    \\ TRY (pairarg_tac \\ fs []) \\ fs [case_eq_thms] \\ rw []
+    \\ cheat (* TODO ASSUME *)
+   )
+  \\ IF_CASES_TAC \\ fs []
+  >- (* axiom *)
+   (
+    fs [case_eq_thms] \\ rw []
+    \\ TRY (pairarg_tac \\ fs []) \\ fs [case_eq_thms] \\ rw []
+    \\ TRY (pairarg_tac \\ fs []) \\ fs [case_eq_thms] \\ rw []
+    \\ cheat (* TODO find_axiom *)
+   )
+  \\ IF_CASES_TAC \\ fs []
+  >- (* betaConv *)
+   (
+    fs [case_eq_thms] \\ rw []
+    \\ TRY (pairarg_tac \\ fs []) \\ fs [case_eq_thms] \\ rw []
+    \\ cheat (* TODO BETA *)
+   )
+  \\ IF_CASES_TAC \\ fs []
+  >- (* cons *)
+   (fs [case_eq_thms] \\ rw []
+    \\ TRY (pairarg_tac \\ fs []) \\ fs [case_eq_thms] \\ rw []
+    \\ TRY (pairarg_tac \\ fs []) \\ fs [case_eq_thms] \\ rw []
+    \\ map_every imp_res_tac [pop_thm, getList_thm] \\ fs []
+    \\ irule push_thm
+    \\ fs [OBJ_def]
+    \\ metis_tac [])
+  \\ IF_CASES_TAC \\ fs []
+  >- (* const *)
+   (fs [case_eq_thms] \\ rw []
+    \\ TRY (pairarg_tac \\ fs []) \\ fs [case_eq_thms] \\ rw []
+    \\ map_every imp_res_tac [pop_thm, getName_thm] \\ fs []
+    \\ irule push_thm \\ fs [OBJ_def])
+  \\ IF_CASES_TAC \\ fs []
+  >- (* constTerm *)
+   (
+    fs [case_eq_thms] \\ rw []
+    \\ TRY (pairarg_tac \\ fs []) \\ fs [case_eq_thms] \\ rw []
+    \\ TRY (pairarg_tac \\ fs []) \\ fs [case_eq_thms] \\ rw []
+    \\ every_case_tac \\ fs [] \\ rw []
+    \\ TRY (map_every imp_res_tac [pop_thm, getType_thm, getConst_thm] \\ fs [] \\ NO_TAC)
+    \\ TRY (irule push_thm \\ fs [OBJ_def])
+    \\ cheat (* TODO *)
+   )
+  \\ IF_CASES_TAC \\ fs []
+  >- (* deductAntysim *)
+   (
+    fs [case_eq_thms] \\ rw []
+    \\ TRY (pairarg_tac \\ fs []) \\ fs [case_eq_thms] \\ rw []
+    \\ TRY (pairarg_tac \\ fs []) \\ fs [case_eq_thms] \\ rw []
+    \\ cheat (* TODO DEDUCT_ANTISYM_RULE *)
+   )
+  \\ IF_CASES_TAC \\ fs []
+  >- (* def *)
+   (fs [case_eq_thms] \\ rw []
+    \\ fs [insert_dict_def]
+    \\ TRY (pairarg_tac \\ fs []) \\ fs [case_eq_thms, bool_case_eq, COND_RATOR] \\ rw []
+    \\ map_every imp_res_tac [pop_thm, peek_thm, getNum_thm] \\ fs []
+    \\ fs [READER_STATE_def])
+  \\ IF_CASES_TAC \\ fs []
+  >- (* defineConst *)
+   (
+    fs [case_eq_thms] \\ rw []
+    \\ TRY (pairarg_tac \\ fs []) \\ fs [case_eq_thms] \\ rw []
+    \\ TRY (pairarg_tac \\ fs []) \\ fs [case_eq_thms] \\ rw []
+    \\ map_every imp_res_tac [getTerm_thm, pop_thm] \\ fs []
+    \\ cheat (* TODO *)
+   )
+  \\ IF_CASES_TAC \\ fs []
+  >- (* defineConstList *)
+    cheat
+  \\ IF_CASES_TAC \\ fs []
+  >- (* defineTypeOp *)
+    cheat
+  \\ IF_CASES_TAC \\ fs []
+  >- (* eqMp *)
+   (fs [case_eq_thms] \\ rw []
+    \\ TRY (pairarg_tac \\ fs []) \\ fs [case_eq_thms] \\ rw []
+    \\ TRY (pairarg_tac \\ fs []) \\ fs [case_eq_thms] \\ rw []
+    \\ map_every imp_res_tac [pop_thm, getThm_thm, EQ_MP_STATE] \\ fs [] \\ rfs []
+    \\ irule push_thm \\ fs [OBJ_def]
+    \\ metis_tac [EQ_MP_thm])
+  \\ IF_CASES_TAC \\ fs []
+  >- (* hdTl *)
+   (fs [case_eq_thms] \\ rw []
+    \\ TRY (pairarg_tac \\ fs []) \\ fs [case_eq_thms] \\ rw []
+    \\ every_case_tac \\ fs [] \\ rw []
+    \\ map_every imp_res_tac [pop_thm, getList_thm] \\ fs []
+    \\ irule push_thm >- metis_tac [OBJ_def]
+    \\ irule push_thm \\ metis_tac [OBJ_def])
+  \\ IF_CASES_TAC \\ fs []
+  >- (* nil *)
+   (fs [case_eq_thms] \\ rw [] \\ fs []
+    \\ irule push_thm \\ fs [OBJ_def])
+  \\ IF_CASES_TAC \\ fs []
+  >- (* opType *)
+   (
+    fs [case_eq_thms] \\ rw []
+    \\ TRY (pairarg_tac \\ fs []) \\ fs [case_eq_thms] \\ rw []
+    \\ TRY (pairarg_tac \\ fs []) \\ fs [case_eq_thms] \\ rw []
+    \\ TRY (map_every imp_res_tac [pop_thm, getList_thm, getType_thm] \\ fs [] \\ NO_TAC)
+    \\ cheat (* TODO *)
+   )
+  \\ IF_CASES_TAC \\ fs []
+  >- (* pop *)
+   (fs [case_eq_thms] \\ rw []
+    \\ TRY (pairarg_tac \\ fs []) \\ fs [case_eq_thms] \\ rw []
+    \\ imp_res_tac pop_thm \\ fs [])
+  \\ IF_CASES_TAC \\ fs []
+  >- (* pragma *)
+   (fs [case_eq_thms] \\ rw []
+    \\ TRY (pairarg_tac \\ fs []) \\ fs [case_eq_thms] \\ rw []
+    \\ imp_res_tac pop_thm \\ fs [])
+  \\ IF_CASES_TAC \\ fs []
+  >- (* proveHyp *)
+   (fs [case_eq_thms] \\ rw []
+    \\ TRY (pairarg_tac \\ fs []) \\ fs [case_eq_thms] \\ rw []
+    \\ TRY (pairarg_tac \\ fs []) \\ fs [case_eq_thms] \\ rw []
+    \\ map_every imp_res_tac [PROVE_HYP_thm, pop_thm, getThm_thm] \\ fs []
+    \\ TRY (irule push_thm \\ fs [OBJ_def])
+    \\ metis_tac [])
+  \\ IF_CASES_TAC \\ fs []
+  >- (* ref *)
+   (
+    fs [case_eq_thms] \\ rw []
+    \\ TRY (pairarg_tac \\ fs []) \\ fs [case_eq_thms, bool_case_eq, COND_RATOR] \\ rw []
+    \\ every_case_tac \\ fs [] \\ rw []
+    \\ map_every imp_res_tac [pop_thm, getNum_thm] \\ fs []
+    \\ irule push_thm \\ fs [OBJ_def]
+    \\ cheat (* TODO need to ensure the dict contains OBJ things *)
+   )
+  \\ IF_CASES_TAC \\ fs []
+  >- (* refl *)
+   (fs [case_eq_thms] \\ rw []
+    \\ TRY (pairarg_tac \\ fs []) \\ fs [case_eq_thms] \\ rw []
+    \\ map_every imp_res_tac [pop_thm, getTerm_thm, REFL_thm] \\ fs []
+    \\ TRY (irule push_thm \\ fs [OBJ_def])
+    \\ metis_tac [])
+  \\ IF_CASES_TAC \\ fs []
+  >- (* remove *)
+   (
+    fs [case_eq_thms] \\ rw []
+    \\ TRY (pairarg_tac \\ fs []) \\ fs [case_eq_thms, bool_case_eq, COND_RATOR] \\ rw []
+    \\ every_case_tac \\ fs [] \\ rw []
+    \\ map_every imp_res_tac [pop_thm, getNum_thm] \\ fs []
+    \\ irule push_thm \\ fs [OBJ_def]
+    \\ cheat (* TODO dicts again *)
+   )
+  \\ IF_CASES_TAC \\ fs []
+  >- (* subst *)
+   (
+    fs [case_eq_thms] \\ rw []
+    \\ TRY (pairarg_tac \\ fs []) \\ fs [case_eq_thms, bool_case_eq, COND_RATOR] \\ rw []
+    \\ TRY (pairarg_tac \\ fs []) \\ fs [case_eq_thms, bool_case_eq, COND_RATOR] \\ rw []
+    \\ TRY (pairarg_tac \\ fs []) \\ fs [case_eq_thms, bool_case_eq, COND_RATOR] \\ rw []
+    \\ map_every imp_res_tac [pop_thm, getThm_thm, getPair_thm, getList_thm] \\ fs []
+    \\ cheat (* TODO *)
+   )
+  \\ IF_CASES_TAC \\ fs []
+  >- (* sym *)
+   (fs [case_eq_thms] \\ rw []
+    \\ TRY (pairarg_tac \\ fs []) \\ fs [case_eq_thms] \\ rw []
+    \\ map_every imp_res_tac [pop_thm, getThm_thm] \\ fs []
+    \\ TRY (irule push_thm \\ fs [OBJ_def])
+    \\ metis_tac [SYM_thm])
+  \\ IF_CASES_TAC \\ fs []
+  >- (* thm *)
+   (
+    fs [case_eq_thms] \\ rw []
+    \\ TRY (pairarg_tac \\ fs []) \\ fs [case_eq_thms] \\ rw []
+    \\ TRY (pairarg_tac \\ fs []) \\ fs [case_eq_thms] \\ rw []
+    \\ TRY (pairarg_tac \\ fs []) \\ fs [case_eq_thms] \\ rw []
+    \\ cheat (* TODO maps *)
+   )
+  \\ IF_CASES_TAC \\ fs []
+  >- (* trans *)
+   (fs [case_eq_thms] \\ rw []
+    \\ TRY (pairarg_tac \\ fs []) \\ fs [case_eq_thms] \\ rw []
+    \\ TRY (pairarg_tac \\ fs []) \\ fs [case_eq_thms] \\ rw []
+    \\ map_every imp_res_tac [pop_thm, getThm_thm] \\ fs []
+    \\ TRY (irule push_thm \\ fs [OBJ_def])
+    \\ metis_tac [TRANS_thm])
+  \\ IF_CASES_TAC \\ fs []
+  >- (* typeOp *)
+   (fs [case_eq_thms] \\ rw []
+    \\ TRY (pairarg_tac \\ fs []) \\ fs [case_eq_thms] \\ rw []
+    \\ map_every imp_res_tac [pop_thm, getName_thm] \\ fs []
+    \\ irule push_thm \\ fs [OBJ_def])
+  \\ IF_CASES_TAC \\ fs []
+  >- (* var *)
+   (fs [case_eq_thms] \\ rw []
+    \\ TRY (pairarg_tac \\ fs []) \\ fs [case_eq_thms] \\ rw []
+    \\ TRY (pairarg_tac \\ fs []) \\ fs [case_eq_thms] \\ rw []
+    \\ map_every imp_res_tac [pop_thm, getName_thm, getType_thm] \\ fs []
+    \\ irule push_thm \\ fs [OBJ_def])
+  \\ IF_CASES_TAC \\ fs []
+  >-
+   (
+    fs [case_eq_thms] \\ rw []
+    \\ TRY (pairarg_tac \\ fs []) \\ fs [case_eq_thms] \\ rw []
+    \\ map_every imp_res_tac [pop_thm, getVar_thm] \\ fs []
+    \\ rename1 `mk_var v1` \\ PairCases_on `v1` \\ fs [mk_var_def, TERM_def]
+    \\ irule push_thm \\ fs [OBJ_def]
+    \\ cheat (* TODO Var .. *)
+   )
+  \\ IF_CASES_TAC \\ fs []
+  >- (* varType *)
+   (fs [case_eq_thms] \\ rw []
+    \\ TRY (pairarg_tac \\ fs []) \\ fs [case_eq_thms] \\ rw []
+    \\ map_every imp_res_tac [pop_thm, getName_thm] \\ fs []
+    \\ irule push_thm \\ fs []
+    \\ fs [OBJ_def, STATE_def]
+    \\ irule mk_vartype_thm
+    \\ metis_tac [STATE_def, CONTEXT_def])
+     (* digits *)
+  \\ every_case_tac \\ fs [] \\ rw [] \\ fs []
+  \\ irule push_thm \\ fs [OBJ_def]);
+
+val readLines_thm = Q.store_thm("readLines_thm",
+  `!lines st res refs refs'.
+     STATE defs refs /\
+     READER_STATE defs st /\
+     readLines lines st refs = (res, refs')
+     ==>
+     STATE defs refs' /\
+     case res of
+       Failure _ => T
+     | Success st' => READER_STATE defs st'`,
+  recInduct readLines_ind \\ once_rewrite_tac [readLines_def] \\ rw []
+  \\ fs [st_ex_return_def, st_ex_bind_def] \\ Cases_on `lls` \\ fs [] \\ rw []
+  \\ Cases_on `t` \\ fs []
+  \\ TRY
+   (fs [Once readLines_def, st_ex_return_def]
+    \\ every_case_tac \\ imp_res_tac readLine_thm \\ fs []
+    \\ rw [] \\ fs []
+    \\ NO_TAC)
+  \\ pop_assum mp_tac
+  \\ CASE_TAC \\ fs []
+  \\ reverse CASE_TAC \\ fs []
+  >- (rw [] \\ metis_tac [readLine_thm])
+  \\ simp [Once readLines_def, st_ex_bind_def]
+  \\ CASE_TAC \\ fs []
+  \\ reverse CASE_TAC \\ fs []
+  >- (rw [] \\ imp_res_tac readLine_thm \\ fs [])
+  \\ strip_tac
+  \\ `STATE defs r /\ READER_STATE defs a` by (imp_res_tac readLine_thm \\ fs [])
+  \\ first_x_assum drule \\ rveq
+  \\ disch_then drule \\ fs [])
+
+val readLines_init_state_thm = Q.store_thm("readLines_init_state_thm",
+  `STATE defs refs /\
+  readLines lines init_state refs = (res, refs')
+  ==>
+  STATE defs refs' /\
+  case res of
+    Failure _ => T
+  | Success st' => READER_STATE defs st'`,
+  sg `READER_STATE defs init_state`
+  >- fs [init_state_def, READER_STATE_def]
+  \\ rw []
+  \\ metis_tac [readLines_thm]);
 
 val _ = export_theory();
 
